### 1. **Solving Systems of Linear Equations by Graphing**

1. Solve the system by graphing:
   $$
   \begin{aligned}
   2x + y &= 4 \\
   x - y &= 1
   \end{aligned}
   $$

2. Solve the system by graphing:
   $$
   \begin{aligned}
   3x + 2y &= 6 \\
   -x + y &= 1
   \end{aligned}
   $$

3. Solve the system by graphing:
   $$
   \begin{aligned}
   x + y &= 3 \\
   x - 2y &= -6
   \end{aligned}
   $$

4. Solve the system by graphing:
   $$
   \begin{aligned}
   4x - y &= 7 \\
   2x + 3y &= 9
   \end{aligned}
   $$

5. Solve the system by graphing:
   $$
   \begin{aligned}
   5x + 4y &= 12 \\
   -3x + 2y &= -6
   \end{aligned}
   $$

---

### 2. **Solving Systems of Linear Equations by Substitution**

6. Solve the system using substitution:
   $$
   \begin{aligned}
   y &= 3x + 1 \\
   2x - y &= 4
   \end{aligned}
   $$

7. Solve the system using substitution:
   $$
   \begin{aligned}
   x &= 2y + 3 \\
   4x - y &= 9
   \end{aligned}
   $$

8. Solve the system using substitution:
   $$
   \begin{aligned}
   x &= 5y + 2 \\
   2x + 3y &= 10
   \end{aligned}
   $$

9. Solve the system using substitution:
   $$
   \begin{aligned}
   y &= 4x - 2 \\
   x + y &= 6
   \end{aligned}
   $$

10. Solve the system using substitution:
   $$
   \begin{aligned}
   2x &= y - 5 \\
   x + 3y &= 8
   \end{aligned}
   $$

---

### 3. **Solving Systems of Linear Equations by Addition**

11. Solve the system using addition:
   $$
   \begin{aligned}
   3x + 2y &= 5 \\
   5x - 2y &= 11
   \end{aligned}
   $$

12. Solve the system using addition:
   $$
   \begin{aligned}
   2x + 3y &= 7 \\
   -4x - 3y &= -9
   \end{aligned}
   $$

13. Solve the system using addition:
   $$
   \begin{aligned}
   x - y &= 1 \\
   2x + y &= 9
   \end{aligned}
   $$

14. Solve the system using addition:
   $$
   \begin{aligned}
   6x + y &= 13 \\
   4x - y &= 1
   \end{aligned}
   $$

15. Solve the system using addition:
   $$
   \begin{aligned}
   x + 2y &= 4 \\
   3x + 2y &= 10
   \end{aligned}
   $$

---

### 4. **Solving Systems of Linear Equations in Three Variables**

16. Solve the system:
   $$
   \begin{aligned}
   x + y + z &= 6 \\
   2x - y + z &= 3 \\
   x + 2y - z &= 2
   \end{aligned}
   $$

17. Solve the system:
   $$
   \begin{aligned}
   3x + 2y + z &= 12 \\
   x - y + 2z &= 4 \\
   2x + 3y - z &= 7
   \end{aligned}
   $$

18. Solve the system:
   $$
   \begin{aligned}
   x + 2y + 3z &= 10 \\
   2x - y + z &= 5 \\
   3x + y - z &= 7
   \end{aligned}
   $$

19. Solve the system:
   $$
   \begin{aligned}
   2x + y + z &= 9 \\
   x - 2y + 3z &= 6 \\
   3x + 2y - z &= 5
   \end{aligned}
   $$

20. Solve the system:
   $$
   \begin{aligned}
   x - y + z &= 3 \\
   2x + y - 2z &= 4 \\
   3x - y + 2z &= 7
   \end{aligned}
   $$

---

### 5. **Systems of Linear Equations and Problem Solving**

21. A person buys 5 apples and 3 oranges for $4.50. Another person buys 7 apples and 4 oranges for $6.10. Determine the cost of one apple and one orange.

22. A chemist mixes two solutions: one contains 30% acid, and the other contains 50% acid. She needs to create 100 liters of a 40% acid solution. How much of each solution should she mix?

23. A company sells two products: one priced at $40 and another priced at $60. In a month, they sell 500 items, making a total of $24,000. How many of each product did they sell?

24. Two trains are 300 miles apart and moving towards each other. One train is moving at 70 miles per hour, and the other is moving at 50 miles per hour. In how many hours will they meet?

25. A person invests $10,000 in two types of bonds: one paying 5% interest and the other paying 7%. At the end of the year, they earned $620 in interest. How much was invested in each bond?

---

### 6. **Exponents**

26. Simplify: $ (x^3)^2 $

27. Simplify: $ (2^4)(2^3) $

28. Simplify: $ (5x^2)(3x^3) $

29. Simplify: $ (3x^4)^2 $

30. Simplify: $ (x^5)(x^2) $

---

### 7. **Polynomial Functions and Adding and Subtracting Polynomials**

31. Add: $ (3x^2 + 2x + 1) + (5x^2 - 3x + 4) $

32. Subtract: $ (7x^3 - 4x^2 + 3) - (2x^3 - 5x^2 + 6) $

33. Add: $ (x^2 + 3x - 4) + (2x^2 - 6x + 8) $

34. Subtract: $ (5x^3 - 2x^2 + 7) - (3x^3 + 6x^2 - 4) $

35. Add: $ (x^4 + 2x^3 + x) + (3x^4 - x^3 + 2x) $

---

### 8. **Multiplying Polynomials**

36. Multiply: $ (x + 3)(x - 4) $

37. Multiply: $ (2x + 5)(x - 3) $

38. Multiply: $ (x^2 - 2x + 1)(x + 1) $

39. Multiply: $ (x^2 + 3x)(x - 2) $

40. Multiply: $ (3x + 2)(x^2 - x + 4) $

---

### 9. **Special Products**

41. Expand: $ (x + 3)^2 $

42. Expand: $ (2x - 5)^2 $

43. Expand: $ (x - 1)^3 $

44. Expand: $ (x + 4)(x - 4) $

45. Expand: $ (x + 5)^2 $

---

### 10. **Negative Exponents and Scientific Notation**

46. Simplify: $ 2^{-3} $

47. Simplify: $ (x^{-2})(x^4) $

48. Write in scientific notation: $ 0.00045 $

49. Write in standard form: $ 5.7 \times 10^3 $

50. Simplify: $ 3^{-2}x^5 $

---

### 11. **Dividing Polynomials**

51. Divide: $ \frac{6x^3 - 9x^2}{3x} $

52. Divide: $ \frac{x^4 + 2x^3 - x}{x} $

53. Divide: $ \frac{10x^2 - 15x}{5x} $

54. Divide: $ \frac{3x^3 - 6x^2 + 9x}{3x} $

55. Divide: $ \frac{x^5 - 3x^3 + x}{x^2} $

---

### 12. **Synthetic Division and the Remainder Theorem**

56. Use synthetic division to divide $ 2x^3 + 3x^2 - 4x + 5 $ by $ x - 2 $.

57. Use synthetic division to divide $ x^3 - 2x^2 + x - 6 $ by $ x + 3 $.

58. Use synthetic division to divide $ 4x^3 + 3x^2 - 2x + 1 $ by $ x - 1 $.

59. Apply the remainder theorem to $ f(x) = x^3 - 5x^2 + 2x - 4 $ for $ x = 2 $.

60. Apply the remainder theorem to $ f(x) = 2x^4 - 3x^3 + 5x - 7 $ for $ x = -1 $.

---

